ViewFunctions.v
@@ -18,10 +18,10 @@ Fixpoint Tuple (d : List nat) : Type :=
   | h::tl => (Idx h) * (Tuple tl)
 end.
 
-Fixpoint ViewArray (s : nat) (d : List nat) :=
+Fixpoint ViewArray (l : nat) (d : List nat) :=
   match d with
-  | [] => Idx s (* Index in the underlying array (s is the size of the array) *)
-  | h::tl => Idx h -> (ViewArray s tl)
+  | [] => Idx l (* Index in the underlying array (s is the size of the array) *)
+  | h::tl => Idx h -> (ViewArray l tl)
 end.
 
 Notation "[[ T ; n ]]" := (n::T).
@@ -32,21 +32,21 @@ Definition identity_view (n : nat) : ViewArray n [[;n]] :=
   i-th element of the view is the i-th element of the array *)
   fun i => idx n (to_nat i) (BoundedInt n i).
 
-Definition reverse {s : nat} {T : List nat} {n : nat} (v : ViewArray s [[T;n]]) : ViewArray s [[T;n]] :=
+Definition reverse {l : nat} {T : List nat} {n : nat} (v : ViewArray l [[T;n]]) : ViewArray l [[T;n]] :=
   fun i => v (idx n (n - 1 - to_nat i) reverseProof).
 
-Definition take_left {s : nat} {T : List nat} {n : nat} (b : nat) (v : ViewArray s [[T;b+n]]) : ViewArray s [[T;b]] :=
+Definition take_left {l : nat} {T : List nat} {n : nat} (b : nat) (v : ViewArray l [[T;b+n]]) : ViewArray l [[T;b]] :=
   fun i => v (idx (b+n) (to_nat i) takeleftProof).
 
-Definition take_right {s : nat} {T : List nat} {n : nat} (a : nat) (v : ViewArray s [[T;a+n]]) : ViewArray s [[T;n]] :=
+Definition take_right {l : nat} {T : List nat} {n : nat} (a : nat) (v : ViewArray l [[T;a+n]]) : ViewArray l [[T;n]] :=
   fun i => v (idx (a+n) (a + to_nat i) takerightProof).
 
-Definition transpose {s : nat} {T : List nat} {n : nat} {m : nat} (v : ViewArray s [[ [[T;m]];n ]]) : ViewArray s [[ [[T;n]];m ]] :=
+Definition transpose {l : nat} {T : List nat} {n : nat} {m : nat} (v : ViewArray l [[ [[T;m]];n ]]) : ViewArray l [[ [[T;n]];m ]] :=
   fun i j => v j i.
 
-Definition group {s : nat} {T : List nat} {n : nat} (m : nat) (v : ViewArray s [[T;m*n]]) : ViewArray s [[ [[T;m]];n]] :=
+Definition group {l : nat} {T : List nat} {n : nat} (m : nat) (v : ViewArray l [[T;m*n]]) : ViewArray l [[ [[T;m]];n]] :=
   fun i j => v (idx (m*n) (to_nat j + m*(to_nat i)) groupProof).
 
-Definition map {s : nat} {A : List nat} {B : List nat} {n : nat} (f : ViewArray s A -> ViewArray s B) (v : ViewArray s [[A;n]]) : ViewArray s [[B;n]] :=
+Definition map {l : nat} {A : List nat} {B : List nat} {n : nat} (f : ViewArray l A -> ViewArray l B) (v : ViewArray l [[A;n]]) : ViewArray l [[B;n]] :=
   fun i => f (v i).
 
